---
title: 'Problem 1'
date: 'October 27,, 2021'
excerpt: 'by: null'
---

Solve:

<br>

`$\frac{1}{x-4}+\frac{1}{x-2}=\frac{2}{x^2-6x+8}$`

<br>

`$\frac{1}{x-4}+\frac{1}{x-2}=\frac{2}{x^2-6x+8}$`

<br>

Restrictions

<br>

`$x\ne2$`

`$x\ne4$`

<br>

`$\frac{1}{x-4}+\frac{1}{x-2}=\frac{2}{(x-2)(x-4)}$`

<br>

`$(x-2)(x-4)(\frac{1}{(x-4)}+\frac{x}{(x-2)})=(\frac{2}{(x-2)(x-4)})(x-2)(x-4)$`

<br>

`$(x-2)+x(x-4)=2$`

<br>

`$x-2+x^2-4x=2$`

<br>

`$x^2-3x-4=0$`

<br>

`$(x-4)(x+1)$`

<br>

`$x-4=0$` or `$x+1=0$`

<br>

`$x=4$` or `$x=-1$`

<br>

Restriction

Solution Set: `$\boxed{\set{-1}}$`



